---
layout: single
title:  "Exercise soln from calculus of variation, Mathematics for Physics"
date : 2023-01-03
header:
  teaser: "unsplash-gallery-image-2-th.jpg"
permalink: /posts/2023/01/blog-post-2/
tags:
  - problems
---
Abstract
===
I am solving the exercise and problems from **chapter 1: calculus of variation** in the following [textbook](https://goldbart.gatech.edu/PostScript/MS_PG_book/bookmaster.pdf):  

Stone, M., & Goldbart, P. (2009). Mathematics for Physics: A Guided Tour for Graduate Students. Cambridge: Cambridge University Press. doi:10.1017/CBO9780511627040


Exercise 1.1
===
A smooth path in the $x$-$y$ plane is given by $\bold r (t)=(x(t),y(t))$ with $\bold r(0)=\bold a$, and $\bold r(1)=\bold b$. The length of the path from $\bold a$ to $\bold b$ is therefore,
$$S[\bold r]=\int_0^1\sqrt{\dot x^2+\dot y^2}dt$$
where $\dot x =dx/dt,\dot y = dy/dt$. Write down the Euler-Lagrange condtions for $S[\bold r]$ to be stationary under small varations of the path that keep the endpoints fixed, and hence show that the shortest path between two points is a straight line. 

Solution
===
The Euler-Lagrange condition is
$$\frac {\partial f}{\partial x}  - \frac d{dt} \left(\frac {\partial f} {\partial \dot x} \right) = 0$$
$$ \frac {\partial f}{\partial y} - \frac d{dt} \left( \frac {\partial f} {\partial \dot y}\right) = 0$$
This translates to the first integrals 
$$ f-\dot x  \frac {\partial f} {\partial \dot x} = const$$
$$ f-\dot y  \frac {\partial f} {\partial \dot y} = const$$
Substitute $f(x,y,\dot x, \dot y) = \sqrt{\dot x ^2 + \dot y^2}$, we have
$$ \sqrt{\dot x ^2 + \dot y^2}-\frac {\dot x^2}{\sqrt{\dot x ^2 + \dot y^2}} = const$$
$$ \sqrt{\dot x ^2 + \dot y^2}-\frac {\dot y^2}{\sqrt{\dot x ^2 + \dot y^2}} = const$$
These imply that both $\dot x$ and $\dot y$ are constants. Thus, both $x$ and $y$ are linear function in terms of time. In order to satisfy the boundary conditions, it must be that 
$$\bold r(t)=(1-t)\bold a + t\bold b$$


Exercise 1.2
===

Solution
===
The Euler-Lagrange condition is
$$\frac {\partial f}{\partial y}  - \frac d{dx} \left(\frac {\partial f} {\partial y'} \right) = 0$$
which translate to
$$\frac d{dx}\left(n(x) \frac {y'}{\sqrt{1+y'^2}}\right) =0$$
Therefore, the Snell's law follows
$$n(x)\sin\psi=const$$
where, $\sin\psi=\frac {y'}{\sqrt{1+y'^2}}$

For the second formula, the first integral is 
$$\frac d{dx} \left(f-y'\frac {\partial f}{\partial y'}\right)=0$$
we have
$$\frac d{dx}\left(n(y)\sqrt{1+y'^2}-n(y)\frac {y'^2}{\sqrt{1+y'^2}}\right) = 0$$
after simplification, 
$$\frac d{dx}\left(n(y)\frac 1{\sqrt{1+y'^2}}\right) = 0$$
Therefore, the Snell's law follows
$$n(y) \sin \varphi= const$$
where $\sin \varphi = \frac 1{\sqrt{1+y'^2}}$.

Notice these two formulas are equavalent since 
$$\sin \psi = \cos \varphi$$


Problem 1.3
===
Solution
===
**Part a)**
The first integral is 
$$\frac d{dx} \left( f-y'\frac {\partial f}{\partial y'}\right)=0$$
which translate to 
$$\frac d{dx}\left(\frac{1}{y}\sqrt{1+y'^2}-\frac{1}{y}\frac{y'^2}{\sqrt{1+y'^2}}\right)=0$$
After simplification, we have
$$\frac 1{y\sqrt{1+y'^2}}=\frac 1C$$
where the constant $C>0$ since by assumption $y>0$.  
Rearrange to get the following ODE,
$$y'=\pm\sqrt{\frac{C^2}{y^2}-1}$$  
Solve it by separation of variables,
$$\pm\frac{y}{\sqrt{C^2-y^2}}dy=dx$$
$$\mp\sqrt{C^2-y^2}=x+D$$
$$(x+D)^2+y^2=C^2$$  
which is cleary a circle with center $(-D,0)$ and radius $C$.  
**Part b)**
It suffices to show any pair of distinct points $(x_1,y_1),(x_2,y_2)$ with $x_1 \neq x_2$ on the upper half plane determine a unique semi-circle in the form 
$$(x+D)^2+y^2=C^2$$
Geometrically, if we find the bisector of the line segment linking $(x_1,y_1),(x_2,y_2)$, it will intersect the $x$-axis exactly once, which gives the center of the circle $(-D,0)$  
**Part c)**   
Let's calculate the distance between the point $(x_0,y_0)$ and $(x_1,0)$ where WLOG we assume $-D\le x_0\lt x_1=-D+C$ and $0<y_0\le C$.
$$\int_{x_0}^{x_1}\frac 1{y}\sqrt{1+y'^2}dx$$
Use the relation from part a) that $\sqrt{1+y'^2}=\frac Cy$, we have
$$\int_{x_0}^{x_1}\frac C{y^2}dx=\int_{x_0}^{x_1}\frac C{C^2-(x+D)^2}dx$$
Apply linear substitution $X:=x+D-C$, we have
$$=\int_{x_0+D-C}^{0} \frac C{C^2-(X-C)^2}dX$$
$$=\frac C2\int_{x_0+D-C}^{0} \left(\frac 1X + \frac 1{2C-X}\right)dX$$
from which, the first term of the integrand leads to divergence of the integral.  

From part a) we understand that for any two distinct points, there is a line connecting them. Therefore, there should be two lines passing through point $A$ and being parallel to the line $q$, one linking points $A$ and the left infinity point of $p$, i.e., $(-D-C,0)$ and the other linking points $A$ and the right infinity point of $p$, i.e.,$(-D+C,0)$.  
Further, the line of pencils is easily argued by geometric drawing.

Problem 1.4
===

Solution
===

Since by assumption, the rod is slightly bend, we can approximate the curvature
$$\kappa = \frac {|y''(z)|}{\left(1+[y'(z)]^2\right)^{\frac 32}}\approx |y''(z)|$$
Therefore, we have
$$U[y]=\int_0^L \frac 12 YIy''^2dz$$
**Part a)**  
to be continued

Problem 1.7
===

Solution
===





