---
layout: single
title:  "Proof of Jensen's Key Result"
date : 2023-11-16
header:
  teaser: "unsplash-gallery-image-2-th.jpg"
permalink: /posts/2023/11/blog-post-4/
tags:
  - Research
---

## Preliminaries

### Notations

$$
n _ c:=\frac{\mathbb{E}(G(G-1))}{\mathbb{G}}
$$

$$
\eta:=\frac{\lambda _ {\underline{Z}}}{\lambda _ {\underline{O}}}
$$

$$
k _ O^f=\frac{\int f(t _ {o _ 1},t _ {o _ 2})dM _ {O|o _ 1,o _ 2}^{(2)}(t _ {o _ 1},t _ {o _ 2})}{\int\int f(t _ {o _ 1},t _ {o _ 2})dM _ {O|o _ 1}(t _ {o _ 1})dM _ {O|o _ 2}(t _ {o _ 2})}
$$

$$
\gamma _ 2^O:=\int\int f(t _ {o _ 1},t _ {o _ 2})dM _ {O|o _ 1}(t _ {o _ 1})dM _ {O|o _ 2}(t _ {o _ 2})
$$

$$
\begin{align*}
\gamma _ 2(f):&=\frac{\mathbb{E}\left(\sum _ {i=1}^G\sum _ {i^\prime=1}^{G^\prime}f(t _ {o _ i},t _ {o _ {i^\prime}})\right)}{\mathbb{E}(G)^2}\\
&=\int \int f\left(t _ {z _ i},t _ {z _ {i^\prime}}\right)dM _ Z(t _ {z _ i})dM _ Z(t _ {z _ {i^\prime}})\\
\end{align*}
$$

$$
\gamma _ 2^{EZ}:=\int\int f(t _ {z},t _ {e})dM _ {Z|z}(t _ {z})dM _ {E|e}(t _ {e})
$$

$$
\gamma _ 2^{EE}:=\int\int f(t _ {e _ 1},t _ {e _ 2})dM _ {E|e _ 1}(t _ {e _ 1})dM _ {E|e _ 2}(t _ {e _ 2})
$$

$$
h _ \epsilon \star g _ X(\|y-y^\prime\|) :=\int h _ \epsilon(y-x)h _ \epsilon(y^\prime - x^\prime) g _ X(\|x-x^\prime \|)dxdx^\prime
$$

$$
h _ \epsilon \star h _ \epsilon(\|y-y^\prime\|) :=\int h _ \epsilon(y-x)h _ \epsilon(y^\prime-x)dx
$$

### Some lemmas used in the proof

**Lemma 1**

$$
\gamma _ 2^O(f)=\eta^2\gamma _ 2(f)+2\eta(1-\eta)\gamma _ 2^{EZ}(f)+(1-\eta)^2\gamma _ 2^{EE}(f)
$$

*Proof*: Note that the 1 point mark distribution can be written as

$$
dM _ {O|o}(t _ {o})=\eta dM _ {Z|z}(t _ {z}) + (1-\eta)dM _ {E|e}(t _ {e})
$$

So the product of the independent 1 point mark distribution can be written

$$
\begin{align*}
dM _ {O|o _ 1}(t _ {o _ 1})dM _ {O|o _ 2}(t _ {o _ 2})=&\eta^2 dM _ {Z|z _ 1}(t _ {z _ 1})dM _ {Z|z _ 2}(t _ {z _ 2}) + \eta(1-\eta)dM _ {Z|z}(t _ {z})dM _ {E|e}(t _ {e})\\
+&(1-\eta)\eta dM _ {E|e}(t _ {e})dM _ {Z|z}(t _ {z})+ (1-\eta)^2dM _ {E|e _ 1}(t _ {e _ 1})dM _ {E|e _ 2}(t _ {e _ 2})\\
\end{align*}
$$

Therefore

$$
\begin{align*}
&\gamma _ 2^O(f)\\
&=\int\int f(t _ {o _ 1},t _ {o _ 2})dM _ {O|o _ 1}(t _ {o _ 1})dM _ {O|o _ 2}(t _ {o _ 2})\\
&=\eta^2\int\int f(t _ {z _ 1},t _ {z _ 2})dM _ {Z|z _ 1}(t _ {z _ 1})dM _ {Z|z _ 2}(t _ {z _ 2}) \\
&+\eta(1-\eta)\int\int f(t _ {z},t _ {e})dM _ {Z|z}(t _ {z})dM _ {E|e}(t _ {e})\\
&+(1-\eta)\eta\int\int f(t _ {e},t _ {z})dM _ {E|e}(t _ {e})dM _ {Z|z}(t _ {z})\\
&+(1-\eta)^2\int\int f(t _ {e _ 1},t _ {e _ 2})dM _ {E|e _ 1}(t _ {e _ 1})dM _ {E|e _ 2}(t _ {e _ 2})\\
&=\eta^2\gamma _ 2(f)+2\eta(1-\eta)\gamma _ 2^{EZ}(f)+(1-\eta)^2\gamma _ 2^{EE}(f)
\end{align*}
$$

To reach the last line, we have used the fact that the query function $f$ is symmetric.

**Lemma 2**

$$
\lambda _ {\underline{Z}}(z)=\mathbb{E}(G)\lambda _ X=:\lambda _ {\underline{Z}}
$$

*Proof*:

$$
\begin{align*}
&\int _ A\lambda _ {\underline{Z}}(z)dz\\
&=\mathbb{E}\left(\sum _ {x \in X} \sum _ {y\in \underline{Y _ x}}\mathrm{1} _ A(y)\right)\\
&=\int\int _ A h _ \epsilon(y-x)dy\lambda _ Xdx\mathbb{E}\left(\sum _ {i=1}^G1\right)\\
&=\mathbb{E}(G)\lambda _ X\int _ A\int h _ \epsilon(y-x)dxdy\\
&=\mathbb{E}(G)\lambda _ X\int _ Ady
\end{align*}
$$

Therefore, $\lambda _ {\underline{Z}}=\mathbb{E}(G)\lambda _ X$

**Lemma 3**
Let's Consider the second order factorial intensity measure restricted to a single protein cluster $\Lambda^{(2)} _ {Y _ x}$ and its ground second order factorial intensity measure $\Lambda^{(2)} _ {\underline{Y _ x}}$, then its conditional 2 point mark probability measure $M _ {Y _ x}^{(2)}$ is given as

$$
M _ {Y _ x}^{(2)}(B _ 1\times B _ 2)=\frac{\mathbb{E}\left(\sum _ {i,j=1}^G\mathrm{1}(i\neq j)\mathrm{1} _ {B _ 1\times B _ 2}(t _ {y _ i},t _ {y _ j})\right)}{\mathbb{E}\left(G(G-1)\right)}
$$

*Proof*: By definition, the second order factorial intensity measure is

$$
\begin{align*}
&\Lambda^{(2)} _ {Y _ x}(A _ 1\times A _ 2,B _ 1\times B _ 2)\\
&=\mathbb{E}\left(\sum _ {i,j=1}^G\mathrm{1}(i\neq j)\mathrm{1} _ {A _ 1\times A _ 2}\left(x+\epsilon _ i,x+\epsilon _ j\right)\mathrm{1} _ {B _ 1\times B _ 2}(t _ {y _ i},t _ {y _ j})\right)\\
&=\mathbb{E}\left(\sum _ {i,j=1}^G\mathrm{1}(i\neq j)\mathrm{1} _ {B _ 1\times B _ 2}(t _ {y _ i},t _ {y _ j})\right)\int _ {A _ 1\times A _ 2} h _ {\epsilon}(y _ 1-x)h _ {\epsilon}(y _ 2-x)dy _ 1dy _ 2
\end{align*}
$$

Similarly, the ground second order factorial intensity measure is

$$
\begin{align*}
&\Lambda^{(2)} _ {\underline{Y _ x}}(A _ 1\times A _ 2)\\
&=\mathbb{E}\left(\sum _ {i,j=1}^G\mathrm{1}(i\neq j)\mathrm{1} _ {A _ 1\times A _ 2}\left(x+\epsilon _ i,x+\epsilon _ j\right)\right)\\
&=\mathbb{E}\left(\sum _ {i,j=1}^G\mathrm{1}(i\neq j)\right)\int _ {A _ 1\times A _ 2} h _ {\epsilon}(y _ 1-x)h _ {\epsilon}(y _ 2-x)dy _ 1dy _ 2\\
&=\mathbb{E}\left(G(G-1)\right)\int _ {A _ 1\times A _ 2} h _ {\epsilon}(y _ 1-x)h _ {\epsilon}(y _ 2-x)dy _ 1dy _ 2\\
\end{align*}
$$

By Campbell' theorem, we have

$$
\Lambda^{(2)} _ {Y _ x}(A _ 1\times A _ 2,B _ 1\times B _ 2)=\int _ {A _ 1\times A _ 2}M _ {Y _ x}^{(2)}(B _ 1,B _ 2)d\Lambda^{(2)} _ {\underline{Y _ x}}(y _ 1,y _ 2)
$$

Thus, $M _ {Y _ x}^{(2)}$ is the conditional probability measure of $\Lambda _ {Y _ x}^{(2)}$ given $\Lambda _ {\underline{Y _ x}}^{(2)}$, so

$$
M _ {Y _ x}(B _ 1\times B _ 2)=\frac{\mathbb{E}\left(\sum _ {i,j=1}^G\mathrm{1}(i\neq j)\mathrm{1} _ {B _ 1\times B _ 2}(t _ {y _ i},t _ {y _ j})\right)}{\mathbb{E}\left(G(G-1)\right)}
$$

## Derivation of the expression of $\Lambda^{f} _ {O}$

Now, let's look at the second order factorial moment weighted by the query function $f$, $\Lambda^{f} _ {O}$

$$
\begin{align*}
&\Lambda^{f} _ {O}(A\times A)\\
&=\mathbb{E}\left(\sum _ {(o _ 1,t _ {o _ 1}),(o _ 2,t _ {o _ 2})\in O, (o _ 1,t _ {o _ 1})\neq(o _ 2,t _ {o _ 2})}\mathrm{1} _ {A\times A}(o _ 1,o _ 2)f(t _ {o _ 1},t _ {o _ 2})\right)\\
&=\mathbb{E}\left(\sum _ {x\in X}\sum _ {i=1}^G\sum _ {j=1}^G\mathrm{1}(i\neq j)\mathrm{1} _ {A\times A}\left(x+\epsilon _ 1,x+\epsilon _ 2\right)f(t _ {y _ 1},t _ {y _ 2})\right)\\
&+\mathbb{E}\left(\sum _ {x,x^\prime\in X,x\neq x^\prime}\sum _ {i=1}^G\sum _ {i^\prime=1}^{G^\prime}\mathrm{1} _ {A\times A}\left(x+\epsilon,x^\prime+\epsilon^{\prime}\right)f(t _ {y},t _ {y^\prime})\right)\\
&+\mathbb{E}\left(\sum _ {(z,t _ z)\in Z}\sum _ {(e,t _ e)\in E}\mathrm{1} _ {A\times A}\left(z,e\right)f(t _ {z},t _ e)\right)\\
&+\mathbb{E}\left(\sum _ {(e,t _ e)\in E}\sum _ {(z,t _ z)\in Z}\mathrm{1} _ {A\times A}\left(e,z\right)f(t _ {e},t _ z)\right)\\
&+\mathbb{E}\left(\sum _ {(e _ 1,t _ {e _ 1}),(e _ 2,t _ {e _ 2})\in E,(e _ 1,t _ {e _ 1})\neq (e _ 2,t _ {e _ 2})}\mathrm{1} _ {A\times A}\left(e _ 1,e _ 2\right)f(t _ {e _ 1},t _ {e _ 2})\right)\\
\end{align*}
$$

So $\Lambda^{f} _ {O}(A\times A)$ is a summation of 5 terms. Let's denote them as the I, II, III, IV and V-th terms and simplify term by term. The first term is

$$
\begin{align*}
I&=\mathbb{E}\left(\sum _ {i=1}^G\sum _ {j=1}^G\mathrm{1}(i\neq j)f(t _ {y _ 1},t _ {y _ 2})\right)\int \Lambda^{(2)} _ {\underline{Y _ x}}(A\times A)\lambda _ X(x)dx\\
&=\frac{\mathbb{E}\left(\sum _ {i=1}^G\sum _ {j=1}^G\mathrm{1}(i\neq j)f(t _ {y _ 1},t _ {y _ 2})\right)}{\mathbb{E}(G(G-1))}\mathbb{E}(G(G-1))\int \Lambda^{(2)} _ {\underline{Y _ x}}(A\times A)\lambda _ X(x)dx\\
&=\gamma _ 1(f)\mathbb{E}(G(G-1))\lambda _ X\int \int _ {A\times A} h _ \epsilon(y-x)h _ \epsilon(y^\prime-x)dydy^\prime dx\\
&=\gamma _ 1(f)\frac{\mathbb{E}(G(G-1))}{\mathbb{E}(G)}\lambda _ {\underline{Z}}\int _ {A\times A}\int h _ \epsilon(y-x)h _ \epsilon(y^\prime-x)dxdydy^\prime\\
&=\gamma _ 1(f)n _ c\lambda _ {\underline{Z}}\int _ {A\times A} h _ \epsilon \star h _ \epsilon(\|y-y^\prime\|) dydy^\prime\\
\end{align*}
$$

The second term is

$$
\begin{align*}
II&=\mathbb{E}\left(\sum _ {i=1}^G\sum _ {i^\prime=1}^{G^\prime}f(t _ {y},t _ {y^\prime})\right)\int\Lambda _ {\underline{Y _ x}}(A)\Lambda _ {\underline{Y _ {x^\prime}}}(A)\lambda^{(2)} _ {X}(x,x^\prime)dxdx^\prime\\
&=\frac{\mathbb{E}\left(\sum _ {i=1}^G\sum _ {i^\prime=1}^{G^\prime}f(t _ {y},t _ {y^\prime})\right)}{\mathbb{E}(G)^2}\mathbb{E}(G)^2\\
&\times \int\Lambda _ {\underline{Y _ x}}(A)\Lambda _ {\underline{Y _ {x^\prime}}}(A)g _ X(\|x-x^\prime \|)\lambda _ X(x)\lambda _ X(x^\prime)dxdx^\prime\\
&=\gamma _ 2(f)\mathbb{E}(G)^2\times \lambda _ X^2\int \int _ {A\times A} h _ \epsilon(y-x)h _ \epsilon(y^\prime - x^\prime)dydy^\prime g _ X(\|x-x^\prime \|)dxdx^\prime\\
&=\gamma _ 2(f)\lambda _ {\underline{Z}}^2 \int _ {A\times A} \int h _ \epsilon(y-x)h _ \epsilon(y^\prime - x^\prime) g _ X(\|x-x^\prime \|)dxdx^\prime dydy^\prime\\
&=\gamma _ 2(f)\lambda _ {\underline{Z}}^2 \int _ {A\times A} h _ \epsilon \star g _ X(\|y-y^\prime\|) dydy^\prime\\
\end{align*}
$$

By symmetry, the third term and the fourth term are identical, therefore

$$
\begin{align*}
III+IV&=2\int f(t _ z,t _ e)dM _ Z(t _ z)dM _ E(t _ e)\int\lambda _ {\underline{Z}}(z)\lambda _ {\underline{E}}(e)dzde\\
&=2\gamma _ 2^{EZ}\lambda _ {\underline{Z}}\lambda _ {\underline{E}}\int _ {A\times A}dzde
\end{align*}
$$

The fifth term is

$$
\begin{align*}

V&=\int f(t _ e,t _ {e^\prime})dM _ Z(t _ e)dM _ E(t _ {e^\prime})\int\lambda _ {\underline{E}}(e)\lambda _ {\underline{E}}(e^\prime)dede^\prime\\
&=\gamma _ 2^{EE}\lambda _ {\underline{E}}^2\int _ {A\times A}dede^\prime
\end{align*}
$$

In summary, we have

$$
\begin{align*}
&\Lambda^{f} _ {O}(A\times A)\\
&=\gamma _ 1(f)n _ c\lambda _ {\underline{Z}}\int _ {A\times A} h _ \epsilon \star h _ \epsilon(\|y-y^\prime\|) dydy^\prime\\
&+\gamma _ 2(f)\lambda _ {\underline{Z}}^2 \int _ {A\times A} h _ \epsilon \star g(\|y-y^\prime\|) dydy^\prime\\
&+2\gamma _ 2^{EZ}\lambda _ {\underline{Z}}\lambda _ {\underline{E}}\int _ {A\times A}dzde\\
&+\gamma _ 2^{EE}\lambda _ {\underline{E}}^2\int _ {A\times A}dede^\prime\\
\end{align*}
$$

By taking the Radon-Nikodym derivative of $\Lambda^{f} _ {O}$ over the product Lebesgue measure $m^2$,

$$
\begin{align*}
&\frac{\partial\Lambda _ O^f}{\partial m^2}(o _ 1,o _ 2)\\
&=\gamma _ 1(f)n _ c\lambda _ {\underline{Z}} h _ \epsilon \star h _ \epsilon(\|y-y^\prime\|)\\
&+\gamma _ 2(f)\lambda _ {\underline{Z}}^2 h _ \epsilon \star g _ X(\|y-y^\prime\|)\\
&+2\gamma _ 2^{EZ}\lambda _ {\underline{Z}}\lambda _ {\underline{E}}\\
&+\gamma _ 2^{EE}\lambda _ {\underline{E}}^2\\
&=\gamma _ 1(f)n _ c\lambda _ {\underline{Z}} h _ \epsilon \star h _ \epsilon(r)+\gamma _ 2(f)\lambda _ {\underline{Z}}^2 h _ \epsilon \star g _ X(r)+2\gamma _ 2^{EZ}\lambda _ {\underline{Z}}\lambda _ {\underline{E}}+\gamma _ 2^{EE}\lambda _ {\underline{E}}^2\\
&=:\frac{\partial\Lambda _ O^f}{\partial m^2}(r)\\
\end{align*}
$$

Notice that this derivative is in terms of $r=\|o _ 1,o _ 2\|$ only.

## Derivation of another expression of $\Lambda^{f} _ {O}$

By Campbell's Theorem, we also know that

$$
\begin{align*}
&\Lambda _ O^f(A\times A)\\
&=\mathbb{E}\left(\sum _ {(o _ 1,t _ {o _ 1}),(o _ 2,t _ {o _ 2})\in O, (o _ 1,t _ {o _ 1})\neq(o _ 2,t _ {o _ 2})}\mathrm{1} _ {A\times A}(o _ 1,o _ 2)f(t _ {o _ 1},t _ {o _ 2})\right)\\
&=\int _ {A\times A} \int f(t _ {o _ 1},t _ {o _ 2})dM _ {O|o _ 1,o _ 2}^{(2)}(t _ {o _ 1},t _ {o _ 2})d\Lambda _ {\underline{O}}^{(2)}(o _ 2,o _ 2)\\
&=\int _ {A\times A} \lambda _ {\underline{O}}^{(2)}(o _ 2,o _ 2)do _ 1do _ 2\int f(t _ {o _ 1},t _ {o _ 2})dM _ {O}^{(2)}(t _ {o _ 1},t _ {o _ 2})\\
\end{align*}
$$

To reach the last line, we have used the fact the 2 point mark distribution is independent of the pair of positions $o _ 1,o _ 2$.

We get another expression for the Radon-Nikodym derivative

$$
\begin{align*}
&\frac{\partial\Lambda _ O^f}{\partial m^2}(o _ 1,o _ 2)\\
&=\lambda _ {\underline{O}}^{(2)}(o _ 2,o _ 2)\int f(t _ {o _ 1},t _ {o _ 2})dM _ {O}^{(2)}(t _ {o _ 1},t _ {o _ 2})\\
&=\lambda _ {\underline{O}}^{(2)}(o _ 2,o _ 2)k _ O^f(o _ 1,o _ 2)\gamma _ 2^O(f)\\
&=\lambda _ {\underline{O}}(o _ 1)\lambda _ {\underline{O}}(o _ 2)g(o _ 2,o _ 2)k _ O^f(o _ 1,o _ 2)\gamma _ 2^O(f)\\
&=\lambda _ {\underline{O}}^2g(\|o _ 1-o _ 2\|)k _ O^f(\|o _ 1-o _ 2\|)\gamma _ 2^O(f)\\
&=\lambda _ {\underline{O}}^2g(r)k _ O^f(r)\gamma _ 2^O(f)\\
&=:\frac{\partial\Lambda _ O^f}{\partial m^2}(r)
\end{align*}
$$

Again the derivative is only dependent on $r:=\|o _ 1-o _ 2\|$.

## Derivation of Jensen's Result

Now we have two expressions for $\Lambda _ O^f$, they have to be equal

$$
\lambda _ {\underline{O}}^2g(r)k _ O^f(r)\gamma _ 2^O(f)=\gamma _ 1(f)n _ c\lambda _ {\underline{Z}} h _ \epsilon \star h _ \epsilon(r)+\gamma _ 2(f)\lambda _ {\underline{Z}}^2 h _ \epsilon \star g _ X(r)+2\gamma _ 2^{EZ}\lambda _ {\underline{Z}}\lambda _ {\underline{E}}+\gamma _ 2^{EE}\lambda _ {\underline{E}}^2
$$

This is simplified to

$$
g(r)k _ O^f(r)\gamma _ 2^O(f)=\gamma _ 1(f)n _ c\frac{\eta}{\lambda _ {\underline{O}}} h _ \epsilon \star h _ \epsilon(r)+\gamma _ 2(f)\eta^2 h _ \epsilon \star g _ X(r)+2\gamma _ 2^{EZ}\eta(1-\eta)+\gamma _ 2^{EE}(1-\eta)^2
$$

Using the fact that $\gamma _ 2^O(f)=\eta\gamma _ 2(f)+2\eta(1-\eta)\gamma _ 2^{EZ}(f)+(1-\eta)^2\gamma _ 2^{EE}(F)$, we have

$$
g(r)k _ O^f(r)\gamma _ 2^O(f)=\gamma _ 1(f)n _ c\frac{\eta}{\lambda _ {\underline{O}}} h _ \epsilon \star h _ \epsilon(r)+\gamma _ 2(f)\eta^2 (h _ \epsilon \star g _ X(r)-1)+\gamma _ 2^O(f)
$$

Since this expression is valid for any query function, if we choose $f=1$, then $k _ O^f(r)=1$, $\gamma _ 2^O(f)=1$, $\gamma _ 1(f)=1$ and $\gamma _ 2(f)=1$. We have

$$
g(r)=n _ c\frac{\eta}{\lambda _ {\underline{O}}} h _ \epsilon \star h _ \epsilon(r)+\eta^2 (h _ \epsilon \star g _ X(r)-1)+1
$$

By rearranging the above expression, we have

$$
\eta^2 (h _ \epsilon \star g _ X(r)-1)=g(r)-n _ c\frac{\eta}{\lambda _ {\underline{O}}} h _ \epsilon \star h _ \epsilon(r)-1
$$

After substituting this equation into the expression of $g(r)k _ O^f(r)\gamma _ 2^O(f)$, we have

$$
g(r)k _ O^f(r)\gamma _ 2^O(f)=(\gamma _ 1(f)-\gamma _ 2(f))n _ c\frac{\eta}{\lambda _ {\underline{O}}} h _ \epsilon \star h _ \epsilon(r)+\gamma _ 2(f)(g(r)-1)+\gamma _ 2^O(f)
$$

## Thoughts

Let's consider the second order factorial ground intensity measure of $O$. The intensity of pair of points $o _ 1,o _ 2$ consists of four parts.

1. The intensity of pairs produced from the same integrin site.
2. The intensity of pairs coming from two distinct integrin sites.
3. The intensity of pairs composed of one from the integrin site and a background noise.
4. The intensity of pairs composed of two background noises.

Therefore,

$$
\begin{aligned}
&\lambda _ {\underline{O}}^{(2)}(o _ 1,o _ 2)\\
&=\lambda _ X\mathbb{E}(G(G-1))h _ \epsilon\star h _ \epsilon(\|o _ 1-o _ 2\|)\\
&+\lambda _ X^2\mathbb{E}(G)^2h _ \epsilon\star g _ X(\|o _ 1-o _ 2\|)\\
&+2\lambda _ {\underline{Z}}\lambda _ {\underline{E}}\\
&+\lambda _ {\underline{E}}^2\\
&=:\lambda _ {\underline{O}}^{(2)}(r)
\end{aligned}
$$

The second order factorial ground intensity measure is dependent on the Euclidean distance $r$ only. Now let's work out the pair correlation function $g$.

$$
\begin{aligned}
g(o _ 1,o _ 2)&=\frac{\lambda _ {\underline{O}}^{(2)}(o _ 1,o _ 2)}{\lambda _ {\underline{O}}(o _ 1)\lambda _ {\underline{O}}(o _ 2)}\\
&=\frac{\lambda _ {\underline{O}}^{(2)}(r)}{\lambda _ {\underline{O}}^2}\\
&=n _ c\frac{\eta}{\lambda _ {\underline{O}}} h _ \epsilon \star h _ \epsilon(r)+\eta^2 h _ \epsilon \star g _ X(r)+2\eta(1-\eta)+(1-\eta)^2\\
&=n _ c\frac{\eta}{\lambda _ {\underline{O}}} h _ \epsilon \star h _ \epsilon(r)+\eta^2 (h _ \epsilon \star g _ X(r)-1)+1
\end{aligned}
$$

The pcf is dependent on the Euclidean distance only, too. It is not hard to see that Jensen's result is a generalization of this in terms of any symmetric query function $f$. When $f=1$, we recover the expression for $g(r)$ from Jensen's result.

Again it is not hard to see this quantity consists of 4 terms. Therefore,

$$
\begin{aligned}
&g(r)k _ O^f(r)\gamma _ 2^O(f)\\
&=n _ c\frac{\eta}{\lambda _ {\underline{O}}} h _ \epsilon \star h _ \epsilon(r)\gamma _ 1(f)\\
&+\eta^2 h _ \epsilon \star g _ X(r)\gamma _ 2(f)\\
&+2\eta(1-\eta)\gamma _ 2^{EZ}(f)\\
&+(1-\eta)^2\gamma _ 2^{EE}(f)
\end{aligned}
$$
