---
layout: single
title:  "The logistic equation and its variant with harvesting"
date : 2023-02-28
header:
  teaser: "unsplash-gallery-image-2-th.jpg"
permalink: /posts/2023/02/blog-post-3/
tags:
  - problems
---

# The logistic differential equation

## The General Solution

Recall the logistic differential equation we learned in Math 100,

$$\frac{dy}{dt} = y(1 - y)$$

Now in Math 101, you just acquired the necessary machinery to solve it
analytically. It can be solved via the separation of variables as
follows:

$$\frac{1}{y(1 - y)}dy = dt$$

$$\int \left( \frac{1}{y} + \frac{1}{1 - y} \right) dy = \int dt $$

Below I will provide two methods to solve it.

### Method I

$$\ln{|y|} - \ln|1 - y| = t + C$$

$$\ln\left| \frac{y}{1 - y} \right| = t + C$$

Do not forget the absolute value sign. And if we try to strip it off, we
need to consider two possible scenarios,

$$\frac{y}{1 - y} = \pm e^{t + C}$$

Setting $B = \pm e^{C}$. Notice this constant $B$ captures both
scenarios.

$$\frac{y}{1 - y} = Be^{t}$$

$$y = \frac{Be^{t}}{1 + Be^{t}}$$

Dividing both numerator and denominator by $Be^{t}$ and set
$A = \frac{1}{B}$, we reach the general solution to the logistic
differential equation,

$$y = \frac{1}{1 + Ae^{- t}}$$

### Method II

$$\int_{}^{}{\left( - \frac{1}{y} - \frac{1}{1 - y} \right)dy} = \int_{}^{}{- dt}$$

$$- \ln|y| + \ln|1 - y| = - t + C$$

$$\ln\left| \frac{1 - y}{y} \right| = - t + C$$

$$\left| \frac{1}{y} - 1 \right| = e^{C}e^{- t}$$

Do not forget the absolute value sign. And if we try to strip it off, we
need to consider two possible scenarios,

$$\frac{1}{y} - 1 = \pm e^{C}e^{- t}$$

$$\frac{1}{y} = 1 \pm e^{C}e^{- t}$$

$$y = \frac{1}{1 \pm e^{C}e^{- t}}$$

Replacing the constant $\pm e^{C}$ with $A$, we reach the general
solution

$$y = \frac{1}{1 + Ae^{- t}}$$

## The Particular Solution

Give the initial condition $y(0) = y_{0}$, we can solve the particular
value of $A$.

$$y_{0} = \frac{1}{1 + A}$$

$$A = \frac{1}{y_{0}} - 1$$

Hence the particular solution is,

$$y = \frac{1}{1 + \left( \frac{1}{y_{0}} - 1 \right)e^{- t}}$$

We will consider sketching the graph of this solution when $y_{0} > 0$
since only positive initial value makes sense in population modelling.
Interested reader can extend to the scenario where $y_{0} = 0$ and
$y_{0} < 0$.

<iframe src="https://www.desmos.com/calculator/mriwg9jjnd?embed" width="500" height="500" style="border: 1px solid #ccc" frameborder=0></iframe>

# The logistic differential equation with proportional harvesting

## The General Solution

Let's turn to the logistic equation with constant proportional
harvesting $ky$ where the constant $k$ represents the per capita
harvesting rate (fishing/hunting/gathering) at a particular $t$,

$$\frac{dy}{dt} = y(1 - k - y)$$

$$\frac{1}{y(1 - k - y)}dy = dt$$

Split the fraction by the method of partial fraction, we have,

$$\frac{1}{1 - k}\int_{}^{}{\left( \frac{1}{y} + \frac{1}{1 - k - y} \right)dy} = \int_{}^{}{dt}$$

Notice we implicitly assume $k \neq 1$, otherwise the integrand will
just be $- \frac{1}{y^{2}}$. We will get back to this special case
later.

### Method I

Now let's integrate,
$$\ln\left| \frac{y}{1 - k - y} \right| = (1 - k)t + C$$

$$\frac{y}{1 - k - y} = \pm e^{(1 - k)t}e^{C}$$

Let $B \equiv \pm e^{c}$ and rearrange the equation so that $y$ is the
subject,

$$y = \frac{(1 - k)Be^{(1 - k)t}}{1 + Be^{(1 - k)t}}$$

Let $A \equiv \frac{1}{B}$, divide both numerator and denominator by
$Be^{(1 - k)t}$, we reach,

$$y = \frac{1 - k}{1 + Ae^{- (1 - k)t}}$$

### Method II

$$\int_{}^{}{\left( - \frac{1}{y} - \frac{1}{1 - k - y} \right)dy} = \int_{}^{}{- (1 - k)dt}$$

$$- \ln|y| + \ln|1 - k - y| = - (1 - k)t + C$$

$$\ln\left| \frac{1 - k}{y} - 1 \right| = e^{C}e^{- (1 - k)t}$$

$$\frac{1 - k}{y} - 1 = \pm e^{- (1 - k)t + C}$$

$$\frac{1 - k}{y} = 1 \pm e^{C}e^{- (1 - k)t}$$

$$y = \frac{1 - k}{1 \pm e^{C}e^{- (1 - k)t}}$$

Denote $A \equiv \pm e^{C}$, we reach,

$$y = \frac{1 - k}{1 + Ae^{- (1 - k)t}}$$

## The Particular Solution

Given the initial condition $y(0) = y_{0}$,

$$y_{0} = \frac{1 - k}{1 + A}$$

Solve $A$,

$$A = \frac{1 - k}{y_{0}} - 1$$

Hence, the particular solution is

$$y = \frac{1 - k}{1 + \left( \frac{1 - k}{y_{0}} - 1 \right)e^{- (1 - k)t}}$$

In the special case when $k = 1$, the logistic differential equation
with harvesting becomes,

$$\frac{dy}{dt} = y(1 - y) - y$$

which translates to,

$$\frac{dy}{dt} = - y^{2}$$

The general solution in this case is,

$$y = \frac{1}{t + A}$$

The particular solution is,

$$y = \frac{1}{t + \frac{1}{y_{0}}}$$

## Effect of $k$ on the solution

$k\  = \ 1$ is an important parameter value. The qualitative behaviour
of the system is different depending on whether $k\  < \ 1$ (stable
steady state $y\  = \ 1\  - \ k$), $k\  = \ 1$ (population death as
$t \rightarrow \infty$ which is asymptotically like $\frac{1}{t}$),
$k\  > \ 1$ (population death as $t \rightarrow \infty$ which is
asymptotically like $e^{- (1 - k)t}\ $so much faster than $\frac{1}{t}$
). I will leave this to the reader to explore and verify these details
through *desmos*:

<iframe src="https://www.desmos.com/calculator/nb76n4pjth?embed" width="500" height="500" style="border: 1px solid #ccc" frameborder=0></iframe>
